wip

Foundation/Modal/Hilbert2/Basic.lean
@@ -62,9 +62,9 @@ noncomputable def inducition!
   (hMaxm       : ∀ {φ}, (h : φ ∈ H.axioms) → motive φ ⟨maxm h⟩)
   (hMdp        : ∀ {φ ψ}, {hpq : H ⊢! φ ➝ ψ} → {hp : H ⊢! φ} → motive (φ ➝ ψ) hpq → motive φ hp → motive ψ (mdp! hpq hp))
   (hNec        : ∀ {φ}, {hp : H ⊢! φ} → (ihp : motive φ hp) → motive (□φ) (nec! hp))
-  (hSubst      : ∀ {φ} (s : Substitution α), {hp : H ⊢! φ} → (ihp : motive φ hp) → motive (φ⟦s⟧) (subst! s hp))
-  (hImply₁     : ∀ {φ ψ}, motive (φ ➝ ψ ➝ φ) $ ⟨imply₁ φ ψ⟩)
-  (hImply₂     : ∀ {φ ψ χ}, motive ((φ ➝ ψ ➝ χ) ➝ (φ ➝ ψ) ➝ φ ➝ χ) $ ⟨imply₂ φ ψ χ⟩)
+  (hSubst      : ∀ {φ} (s), {hp : H ⊢! φ} → (ihp : motive φ hp) → motive (φ⟦s⟧) (subst! s hp))
+  (hImply₁     : ∀ {φ ψ}, motive (Axioms.Imply₁ φ ψ) $ ⟨imply₁ φ ψ⟩)
+  (hImply₂     : ∀ {φ ψ χ}, motive (Axioms.Imply₂ φ ψ χ) $ ⟨imply₂ φ ψ χ⟩)
   (hElimContra : ∀ {φ ψ}, motive (Axioms.ElimContra φ ψ) $ ⟨ec φ ψ⟩)
   : ∀ {φ}, (d : H ⊢! φ) → motive φ d := by
   intro φ d;
@@ -108,5 +108,126 @@ lemma weakerThan_of_subset_axioms (hSubset : H₁.axioms ⊆ H₂.axioms) : H₁
 
 end Hilbert
 
+
+
+namespace Hilbert
+
+def axiomInstances (H : Hilbert α) : Set (Formula α) := { φ⟦s⟧ | (φ ∈ H.axioms) (s : Substitution α) }
+
+lemma mem_axiomInstances_of_mem_axioms {φ} (h : φ ∈ H.axioms) : φ ∈ H.axiomInstances := by
+  use φ;
+  constructor;
+  . assumption;
+  . use Substitution.id;
+    simp;
+
+inductive Deduction₂ (H : Hilbert α) : (Formula α) → Type _
+  | maxm {φ}      : (φ ∈ H.axiomInstances) → Deduction₂ H φ
+  | mdp {φ ψ}     : Deduction₂ H (φ ➝ ψ) → Deduction₂ H φ → Deduction₂ H ψ
+  | nec {φ}       : Deduction₂ H φ → Deduction₂ H (□φ)
+  | imply₁ φ ψ    : Deduction₂ H $ Axioms.Imply₁ φ ψ
+  | imply₂ φ ψ χ  : Deduction₂ H $ Axioms.Imply₂ φ ψ χ
+  | ec φ ψ        : Deduction₂ H $ Axioms.ElimContra φ ψ
+
+notation H " ⊢² " φ => Deduction₂ H φ
+
+
+def Deductive₂ (H : Hilbert α) (φ) := Nonempty (H ⊢² φ)
+notation H " ⊢²! " φ => Deductive₂ H φ
+
+lemma Deduction₂.nec! {H : Hilbert α} {φ} (h : H ⊢²! φ) : H ⊢²! □φ := ⟨Deduction₂.nec h.some⟩
+
+
+noncomputable def Deduction₂.inducition!
+  {motive      : (φ : Formula α) → (H ⊢²! φ) → Sort*}
+  (hMaxm       : ∀ {φ}, (h : φ ∈ H.axiomInstances) → motive φ ⟨maxm h⟩)
+  (hMdp        : ∀ {φ ψ}, {hpq : H ⊢²! φ ➝ ψ} → {hp : H ⊢²! φ} → motive (φ ➝ ψ) hpq → motive φ hp → motive ψ ⟨mdp hpq.some hp.some⟩)
+  (hNec        : ∀ {φ}, {hp : H ⊢²! φ} → (ihp : motive φ hp) → motive (□φ) ⟨nec hp.some⟩)
+  (hImply₁     : ∀ {φ ψ}, motive (Axioms.Imply₁ φ ψ) $ ⟨imply₁ φ ψ⟩)
+  (hImply₂     : ∀ {φ ψ χ}, motive (Axioms.Imply₂ φ ψ χ) $ ⟨imply₂ φ ψ χ⟩)
+  (hElimContra : ∀ {φ ψ}, motive (Axioms.ElimContra φ ψ) $ ⟨ec φ ψ⟩)
+  : ∀ {φ}, (d : H ⊢²! φ) → motive φ d := by
+  intro φ d;
+  induction d.some with
+  | maxm h => exact hMaxm h
+  | mdp hpq hp ihpq ihp => exact hMdp (ihpq ⟨hpq⟩) (ihp ⟨hp⟩)
+  | nec hp ih => exact hNec (ih ⟨hp⟩)
+  | _ => aesop;
+
+
+lemma deductive₂_of_deductive : H ⊢! φ → H ⊢²! φ := by
+  intro h;
+  induction h using Deduction.inducition! with
+  | hMaxm h => exact ⟨Deduction₂.maxm (mem_axiomInstances_of_mem_axioms (by assumption))⟩;
+  | hMdp ih₁ ih₂ => exact ⟨Deduction₂.mdp ih₁.some ih₂.some⟩;
+  | hNec ih => exact ⟨Deduction₂.nec ih.some⟩;
+  | @hSubst φ s h₁ h₂ => sorry;
+    /-
+    obtain ⟨d₂⟩ := h₂;
+    constructor;
+    cases d₂;
+    . sorry;
+    . sorry;
+    . sorry;
+    . apply Deduction₂.imply₁;
+    . apply Deduction₂.imply₂;
+    . apply Deduction₂.ec;
+    -/
+  | hImply₁ => exact ⟨Deduction₂.imply₁ _ _⟩;
+  | hImply₂ => exact ⟨Deduction₂.imply₂ _ _ _⟩;
+  | hElimContra => exact ⟨Deduction₂.ec _ _⟩;
+
+lemma deductive_of_deductive₂ : (H ⊢²! φ) → (H ⊢! φ) := by
+  intro h;
+  induction h using Deduction₂.inducition! with
+  | hMaxm h =>
+    obtain ⟨ψ, h, ⟨s, rfl⟩⟩ := h;
+    exact Deduction.subst! s $ Deduction.maxm! h;
+  | hMdp ih₁ ih₂ => exact ih₁ ⨀ ih₂;
+  | hNec ih => exact nec! ih;
+  | _ => simp;
+
+theorem iff_deductive_deductive₂ : H ⊢! φ ↔ H ⊢²! φ := ⟨deductive₂_of_deductive, deductive_of_deductive₂⟩
+
+end Hilbert
+
+
+/-
+namespace Hilbert
+
+def Deduction.isSubstless : H ⊢ φ → Prop
+  | subst _ _ => False
+  | _ => True
+
+def SubstlessDeduction (H : Hilbert α) (φ : Formula α) := { d : H ⊢ φ // Deduction.isSubstless d }
+notation H " ⊢ˢ " φ => SubstlessDeduction H φ
+
+open Deduction in
+noncomputable def SubstlessDeduction.rec {motive : Formula α → Sort*}
+  {motive      : (φ : Formula α) → (H ⊢ˢ φ) → Sort*}
+  (hMdp        : ∀ {φ ψ}, {hpq : H ⊢ˢ (φ ➝ ψ)} → {hp : H ⊢ˢ φ} → motive (φ ➝ ψ) hpq → motive φ hp → motive ψ ⟨.mdp hpq.1 hp.1, by simp [isSubstless]⟩)
+  (hNec        : ∀ {φ}, {hp : H ⊢ˢ φ} → (ihp : motive φ hp) → motive (□φ) ⟨.nec hp.1, by simp [isSubstless]⟩)
+  (hImply₁     : ∀ {φ ψ}, motive (φ ➝ ψ ➝ φ) $ ⟨imply₁ φ ψ, by simp [isSubstless]⟩)
+  (hImply₂     : ∀ {φ ψ χ}, motive ((φ ➝ ψ ➝ χ) ➝ (φ ➝ ψ) ➝ φ ➝ χ) $ ⟨imply₂ φ ψ χ, by simp [isSubstless]⟩)
+  (hElimContra : ∀ {φ ψ}, motive (Axioms.ElimContra φ ψ) $ ⟨ec φ ψ, by simp [isSubstless]⟩)
+  : ∀ {φ}, (d : H ⊢ˢ φ) → motive φ d := by
+  rintro φ ⟨d, hd⟩;
+  induction d with
+  | subst s hp ih => simp [isSubstless] at hd;
+  -- | maxm h => exact hMaxm h
+  -- | mdp hpq hp ihpq ihp => exact hMdp (ihpq ⟨hpq⟩) (ihp ⟨hp⟩)
+  | @nec ψ hp ih =>
+    have := ih ?_;
+    have := @hNec ψ;
+    sorry;
+    . sorry;
+  | _ => sorry;
+  -- | _ => aesop;
+
+def SubstlessDeductive (H : Hilbert α) (φ) := Nonempty (SubstlessDeduction H φ)
+notation H:90 " ⊢ˢ! " φ:90 => SubstlessDeductive H φ
+
+end Hilbert
+-/
 
 end LO.Modal
