Foundation/Modal/Kripke2/Basic.lean
@@ -1,7 +1,6 @@
 import Foundation.Vorspiel.RelItr
-import Foundation.Logic.System
-import Foundation.Modal.Formula
-import Foundation.Modal.Hilbert2.Basic
+import Foundation.Modal.Axioms
+import Foundation.Modal.Substitution
 
 namespace LO.Modal
 
@@ -96,6 +95,8 @@ variable {M : Kripke.Model} {x : M.World} {φ ψ : Formula ℕ}
 protected lemma bot_def : ¬x ⊧ ⊥ := by simp [Satisfies];
 
 protected lemma imp_def : x ⊧ φ ➝ ψ ↔ (x ⊧ φ) → (x ⊧ ψ) := by tauto;
+
+protected lemma imp_def₂ : x ⊧ φ ➝ ψ ↔ ¬x ⊧ φ ∨ x ⊧ ψ := by tauto;
 
 protected lemma or_def : x ⊧ φ ⋎ ψ ↔ x ⊧ φ ∨ x ⊧ ψ := by simp [Satisfies]; tauto;
 
@@ -237,6 +238,31 @@ instance : Semantics.Top (Kripke.Frame) where
 instance : Semantics.Bot (Kripke.Frame) where
   realize_bot _ := ValidOnFrame.bot_def
 
+
+lemma iff_not_exists_valuation : (¬F ⊧ φ) ↔ (∃ V : Kripke.Valuation F, ¬(⟨F, V⟩ : Kripke.Model) ⊧ φ) := by
+  simp [ValidOnFrame];
+
+alias ⟨exists_valuation_of_not, not_of_exists_valuation⟩ := iff_not_exists_valuation
+
+
+lemma iff_not_exists_valuation_world : (¬F ⊧ φ) ↔ (∃ V : Kripke.Valuation F, ∃ x : (⟨F, V⟩ : Kripke.Model).World, ¬Satisfies _ x φ) := by
+  simp [ValidOnFrame, Satisfies, ValidOnModel, Semantics.Realize];
+
+alias ⟨exists_valuation_world_of_not, not_of_exists_valuation_world⟩ := iff_not_exists_valuation_world
+
+
+lemma iff_not_exists_model_world :  (¬F ⊧ φ) ↔ (∃ M : Kripke.Model, ∃ x : M.World, M.toFrame = F ∧ ¬(x ⊧ φ)) := by
+  constructor;
+  . intro h;
+    obtain ⟨V, x, h⟩ := iff_not_exists_valuation_world.mp h;
+    use ⟨F, V⟩, x;
+    tauto;
+  . rintro ⟨M, x, rfl, h⟩;
+    exact iff_not_exists_valuation_world.mpr ⟨M.Val, x, h⟩;
+
+alias ⟨exists_model_world_of_not, not_of_exists_model_world⟩ := iff_not_exists_model_world
+
+
 protected lemma mdp (hpq : F ⊧ φ ➝ ψ) (hp : F ⊧ φ) : F ⊧ ψ := by
   intro V x;
   exact (hpq V x) (hp V x);
@@ -245,13 +271,37 @@ protected lemma nec (h : F ⊧ φ) : F ⊧ □φ := by
   intro V x y _;
   exact h V y;
 
-@[simp] protected lemma imply₁ : F ⊧ (Axioms.Imply₁ φ ψ) := by intro V; exact ValidOnModel.imply₁ (M := ⟨F, V⟩);
+protected lemma subst {s : Substitution ℕ} : F ⊧ φ → F ⊧ (φ⟦s⟧) := by
+  contrapose;
+  simp only [iff_not_exists_valuation_world]
+  rintro ⟨V, ⟨x, hx⟩⟩;
+  use (λ x a => x ⊧ a), x;
+  induction φ using Formula.rec' generalizing x with
+  | hatom a => simp_all [Satisfies];
+  | hfalsum => simp [Satisfies];
+  | himp φ ψ ih₁ ih₂ =>
+    apply Satisfies.not_imp.mpr;
+    apply Satisfies.and_def.mpr;
+    have ⟨hφ, hψ⟩ := Satisfies.and_def.mp $ Satisfies.not_imp.mp hx;
+    constructor;
+    . sorry;
+    . apply ih₂;
+      exact hψ;
+  | hbox ψ ih =>
+    simp_all [Satisfies];
+    obtain ⟨y, Rxy, hy⟩ := hx;
+    use y;
+    constructor;
+    . assumption
+    exact ih y hy;
 
-@[simp] protected lemma imply₂ : F ⊧ (Axioms.Imply₂ φ ψ χ) := by intro V; exact ValidOnModel.imply₂ (M := ⟨F, V⟩);
+protected lemma imply₁ : F ⊧ (Axioms.Imply₁ φ ψ) := by intro V; exact ValidOnModel.imply₁ (M := ⟨F, V⟩);
 
-@[simp] protected lemma elimContra : F ⊧ (Axioms.ElimContra φ ψ) := by intro V; exact ValidOnModel.elimContra (M := ⟨F, V⟩);
+protected lemma imply₂ : F ⊧ (Axioms.Imply₂ φ ψ χ) := by intro V; exact ValidOnModel.imply₂ (M := ⟨F, V⟩);
 
-@[simp] protected lemma axiomK : F ⊧ (Axioms.K φ ψ) := by intro V; exact ValidOnModel.axiomK (M := ⟨F, V⟩);
+protected lemma elimContra : F ⊧ (Axioms.ElimContra φ ψ) := by intro V; exact ValidOnModel.elimContra (M := ⟨F, V⟩);
+
+protected lemma axiomK : F ⊧ (Axioms.K φ ψ) := by intro V; exact ValidOnModel.axiomK (M := ⟨F, V⟩);
 
 end ValidOnFrame
 
@@ -303,22 +353,6 @@ lemma iff_not_validOnModel_of_exists_world {M : Kripke.Model} : (¬M ⊧ φ) ↔
 alias ⟨exists_world_of_not_validOnModel_of, not_validOnModel_of_exists_world⟩ := iff_not_validOnModel_of_exists_world
 
 
-lemma iff_not_validOnFrame_exists_valuation_world : (¬F ⊧ φ) ↔ (∃ V : Kripke.Valuation F, ∃ x : (⟨F, V⟩ : Kripke.Model).World, ¬Satisfies _ x φ) := by
-  simp [ValidOnFrame, Satisfies, ValidOnModel, Semantics.Realize];
-
-alias ⟨exists_valuation_world_of_not_validOnFrame_of, not_validOnFrame_of_exists_valuation_world⟩ := iff_not_validOnFrame_exists_valuation_world
-
-lemma iff_not_validOnFrame_exists_model_world :  (¬F ⊧ φ) ↔ (∃ M : Kripke.Model, ∃ x : M.World, M.toFrame = F ∧ ¬(x ⊧ φ)) := by
-  constructor;
-  . intro h;
-    obtain ⟨V, x, h⟩ := iff_not_validOnFrame_exists_valuation_world.mp h;
-    use ⟨F, V⟩, x;
-    tauto;
-  . rintro ⟨M, x, rfl, h⟩;
-    exact iff_not_validOnFrame_exists_valuation_world.mpr ⟨M.Val, x, h⟩;
-
-alias ⟨exists_model_world_of_not_validOnFrame_of, not_validOnFrame_of_exists_model_world⟩ := iff_not_validOnFrame_exists_model_world
-
 
 lemma iff_not_validOnFrameClass_exists_frame {C : Kripke.FrameClass} : (¬C ⊧ φ) ↔ (∃ F ∈ C, ¬F ⊧ φ) := by
   apply not_iff_not.mp;
@@ -346,192 +380,5 @@ lemma notValidOnFiniteFrameClass_of_exists_finite_frame {FC : Kripke.FiniteFrame
 
 end Kripke
 
-
--- def Frame.theorems (F : Kripke.Frame) : Theory ℕ := { φ | F ⊧ φ }
-
-/-
-def FrameClass.definedBy (C : Kripke.FrameClass) (Γ : Set (Formula ℕ)) := ∀ F, F ∈ C ↔ F ⊧* Γ
-
-def FrameClass.definedByFormula (C : Kripke.FrameClass) (φ : Formula ℕ) := C.definedBy {φ}
-
-
-def FiniteFrameClass.definedBy (C : Kripke.FiniteFrameClass) (Γ : Set (Formula ℕ)) := ∀ F, F ∈ C ↔ F.toFrame ⊧* Γ
-
-def FiniteFrameClass.definedByFormula (C : Kripke.FiniteFrameClass) (φ : Formula ℕ) := C.definedBy {φ}
-
-
-section definability
-
-variable {C : Kripke.FrameClass} {FC : Kripke.FiniteFrameClass} {Ax : Set (Formula ℕ)}
-
-lemma FiniteFrameClass.definedBy_of_definedBy_frameclass_aux (h : C.definedBy Ax) : (C.restrictFinite).DefinedBy Ax := by
-  intro F;
-  constructor;
-  . intro hF;
-    apply h F.toFrame |>.mp hF;
-  . intro hF;
-    apply h F.toFrame |>.mpr hF;
-
-lemma FiniteFrameClass.definedBy_of_definedBy_frameclass (h : C.DefinedBy Ax) (e : FC = C.restrictFinite) : FC.DefinedBy Ax := by
-  rw [e];
-  exact FiniteFrameClass.definedBy_of_definedBy_frameclass_aux h;
-
-
-lemma AllFrameClass.isDefinedBy : AllFrameClass.DefinedBy 𝗞 := by
-  intro F;
-  simp;
-  rintro _ φ ψ rfl;
-  exact Formula.Kripke.ValidOnFrame.axiomK;
-
-lemma AllFiniteFrameClass.isDefinedBy : AllFiniteFrameClass.DefinedBy 𝗞 := FiniteFrameClass.definedBy_of_definedBy_frameclass AllFrameClass.isDefinedBy $ by rfl
-
-end definability
-
-
-end Kripke
-
-
-namespace Hilbert
-
-open Kripke
-
-namespace Kripke
-
-variable {H : Hilbert ℕ} {φ : Formula ℕ}
-variable {T : Set (Formula ℕ)}
-
-open Formula.Kripke
-
-section
-
-variable {C : FrameClass} {H : Hilbert ℕ}
-
-lemma instSound_of_frameClass_definedBy_aux (definedBy : C.DefinedBy T) (ha : H.axioms ⊆ T) : H ⊢! φ → C ⊧ φ := by
-  intro hφ F hF;
-  induction hφ using Hilbert.Deduction.inducition! with
-  | hImply₁ => apply ValidOnFrame.imply₁;
-  | hImply₂ => apply ValidOnFrame.imply₂;
-  | hElimContra => apply ValidOnFrame.elimContra;
-  | hMdp ihpq ihp => exact ValidOnFrame.mdp ihpq ihp;
-  | hNec ih => exact ValidOnFrame.nec ih;
-  | hSubst => sorry;
-  | hMaxm h =>
-    apply Semantics.realizeSet_iff.mp (definedBy F |>.mp hF);
-    exact ha h;
-
-lemma instSound_of_frameClass_definedBy (definedBy : C.DefinedBy T) (heq : H =ₛ (Hilbert.ExtK T)) : Sound H C := ⟨by
-  intro φ hφ;
-  apply instSound_of_frameClass_definedBy_aux definedBy;
-  exact Equiv.iff.mp heq φ |>.mp hφ;
-⟩
-
-lemma instConsistent_of_nonempty_frameclass_aux [sound : Sound H C] (hNonempty : C.Nonempty) : H ⊬ ⊥ := by
-  apply not_imp_not.mpr sound.sound;
-  simp [Semantics.Realize];
-  obtain ⟨F, hF⟩ := hNonempty;
-  use F;
-  constructor;
-  . exact hF;
-  . exact Semantics.Bot.realize_bot (F := Formula ℕ) (M := Kripke.Frame) F;
-
-lemma instConsistent_of_nonempty_frameclass [Sound H C] (h_nonempty : C.Nonempty) : H.Consistent := System.Consistent.of_unprovable $ instConsistent_of_nonempty_frameclass_aux h_nonempty
-
-end
-
-
-section
-
-variable {FC : FiniteFrameClass}
-
-lemma instSound_of_finiteFrameClass_definedBy_aux (definedBy : FC.DefinedBy T) : (Hilbert.ExtK T : Hilbert ℕ) ⊢! φ → FC ⊧ φ := by
-  intro hφ F hF;
-  obtain ⟨F, hF, rfl⟩ := hF;
-  induction hφ using Hilbert.Deduction.inducition_with_necOnly! with
-  | hImply₁ => apply ValidOnFrame.imply₁;
-  | hImply₂ => apply ValidOnFrame.imply₂;
-  | hElimContra => apply ValidOnFrame.elimContra;
-  | hMdp ihpq ihp => exact ValidOnFrame.mdp ihpq ihp;
-  | hNec ih => exact ValidOnFrame.nec ih;
-  | hMaxm h =>
-    simp at h;
-    rcases h with (⟨_, _, rfl⟩ | hR);
-    . exact Formula.Kripke.ValidOnFrame.axiomK;
-    . apply Semantics.realizeSet_iff.mp (definedBy F |>.mp hF);
-      assumption;
-
-lemma instSound_of_finiteFrameClass_definedBy (definedBy : FC.DefinedBy T) (heq : H =ₛ (Hilbert.ExtK T)) : Sound H FC := ⟨by
-  intro φ hφ;
-  apply instSound_of_finiteFrameClass_definedBy_aux definedBy;
-  exact Equiv.iff.mp heq φ |>.mp hφ;
-⟩
-
-lemma instConsistent_of_nonempty_finiteFrameclass_aux [sound : Sound H FC] (hNonempty : FC.Nonempty) : H ⊬ ⊥ := by
-  apply not_imp_not.mpr sound.sound;
-  simp [Semantics.Realize];
-  obtain ⟨F, hF⟩ := hNonempty;
-  use F.toFrame;
-  constructor;
-  . use F;
-  . exact Semantics.Bot.realize_bot (F := Formula ℕ) (M := Kripke.Frame) F.toFrame;
-
-lemma instConsistent_of_nonempty_finiteFrameclass [Sound H FC] (h_nonempty : FC.Nonempty) : H.Consistent :=
-  System.Consistent.of_unprovable $ instConsistent_of_nonempty_finiteFrameclass_aux h_nonempty
-
-end
-
-lemma instFiniteSound_of_instSound {C : FrameClass} {FC : FiniteFrameClass} (heq : C.restrictFinite = FC) [sound : Sound H C] : Sound H FC := ⟨by
-  intro φ hφ F hF;
-  apply sound.sound (f := φ) hφ;
-  rw [←heq] at hF;
-  simp [FrameClass.restrictFinite, FiniteFrameClass.toFrameClass] at hF;
-  obtain ⟨F, hF, rfl⟩ := hF;
-  exact hF;
-⟩
-
-class FiniteFrameProperty (H : Hilbert ℕ) (FC : FiniteFrameClass) where
-  sound : Sound H FC
-  complete : Complete H FC
-
-end Kripke
-
-
-namespace K
-
-instance Kripke.sound : Sound (Hilbert.K ℕ) (AllFrameClass) := Kripke.instSound_of_frameClass_definedBy (definedBy := Kripke.AllFrameClass.isDefinedBy) (heq := by simp [ExtK.K_is_extK_of_AxiomK])
-
-instance consistent : System.Consistent (Hilbert.K ℕ) := Kripke.instConsistent_of_nonempty_frameclass (C := AllFrameClass) $ by
-  use reflexivePointFrame.toFrame;
-  tauto;
-
-end K
-
-
-section
-
-variable {Ax₁ Ax₂ : Theory ℕ} (C₁ C₂ : FrameClass)
-
-lemma Kripke.weakerThan_of_subset_FrameClass
-  [sound₁ : Sound (Hilbert.ExtK Ax₁) C₁] [complete₂ : Complete (Hilbert.ExtK Ax₂) C₂]
-  (h𝔽 : C₂ ⊆ C₁)
-  : (Hilbert.ExtK Ax₁) ≤ₛ (Hilbert.ExtK Ax₂) := by
-  apply System.weakerThan_iff.mpr;
-  intro φ hp;
-  apply complete₂.complete;
-  intro F hF;
-  exact sound₁.sound hp $ h𝔽 hF;
-
-lemma Kripke.equiv_of_eq_FrameClass
-  [sound₁ : Sound (Hilbert.ExtK Ax₁) C₁] [sound₂ : Sound (Hilbert.ExtK Ax₂) C₂]
-  [complete₁ : Complete (Hilbert.ExtK Ax₁) C₁] [complete₂ : Complete (Hilbert.ExtK Ax₂) C₂]
-  (hC : C₁ = C₂) : (Hilbert.ExtK Ax₁) =ₛ (Hilbert.ExtK Ax₂) := by
-  apply System.Equiv.antisymm_iff.mpr;
-  constructor;
-  . apply weakerThan_of_subset_FrameClass C₁ C₂; subst_vars; rfl;
-  . apply weakerThan_of_subset_FrameClass C₂ C₁; subst_vars; rfl;
-
-end
-
-end Hilbert
--/
 
 end LO.Modal
