Foundation/Modal/Substitution.lean
@@ -2,15 +2,16 @@ import Foundation.Modal.Formula
 
 namespace LO.Modal
 
-abbrev Substitution (α) := α → Modal.Formula α
+abbrev Substitution (α) := α → (Formula α)
 
+abbrev Substitution.id {α} : Substitution α := λ a => .atom a
 
 namespace Formula
 
 variable {φ ψ : Formula α} {s : Substitution α}
 
 def subst (s : Substitution α) : Formula α → Formula α
-  | atom a  => s a
+  | atom a  => (s a)
   | ⊥       => ⊥
   | □φ      => □(φ.subst s)
   | φ ➝ ψ   => φ.subst s ➝ ψ.subst s
@@ -36,6 +37,9 @@ notation:80 φ "⟦" s "⟧" => Formula.subst s φ
 @[simp] lemma subst_dia : (◇φ)⟦s⟧ = ◇(φ⟦s⟧) := rfl
 
 end Formula
+
+
+@[simp] lemma subst_id {φ : Formula α} : φ⟦.id⟧ = φ := by induction φ using Formula.rec' <;> simp_all;
 
 
 class SubstitutionClosed (S : Set (Formula α)) where
