Foundation/Modal/Hilbert2/Geach.lean
@@ -4,51 +4,60 @@ namespace LO.Modal
 
 namespace Hilbert
 
-variable (α) [DecidableEq α] [h2 : HasElements 2 α]
+variable (α) [DecidableEq α]
 
-protected def Geach (G : Set (GeachConfluent.Taple)) : Hilbert α := ⟨
-  {Axioms.K (.atom (h2.vec[0])) (.atom (h2.vec[1]))}
-  ∪ G.image (λ t => Axioms.Geach t (h2.vec[0]))
+protected def Geach (G : Set (GeachConfluent.Taple)) : Hilbert ℕ := ⟨
+  {Axioms.K (.atom 0) (.atom 1)}
+  ∪ G.image (λ t => Axioms.Geach t (.atom 0))
 ⟩
 
-instance HasT_of_mem_0_0_1_0 (h : ⟨0, 0, 1, 0⟩ ∈ G) : HasT (Hilbert.Geach α G) where
-  p := h2.vec[0]
+instance HasT_of_mem_0_0_1_0 (h : ⟨0, 0, 1, 0⟩ ∈ G) : HasT (Hilbert.Geach G) where
+  p := 0
   mem_T := by
-    unfold Hilbert.Geach;
-    simp;
+    simp [Hilbert.Geach];
     use ⟨0, 0, 1, 0⟩;
     simpa;
 
-instance HasB_of_mem_0_1_0_1 (h : ⟨0, 1, 0, 1⟩ ∈ G) : HasB (Hilbert.Geach α G) where
-  p := h2.vec[0]
+instance HasB_of_mem_0_1_0_1 (h : ⟨0, 1, 0, 1⟩ ∈ G) : HasB (Hilbert.Geach G) where
+  p := 0
   mem_B := by
-    unfold Hilbert.Geach;
-    simp;
+    simp [Hilbert.Geach];
     use ⟨0, 1, 0, 1⟩;
     simpa;
 
-instance HasD_of_mem_0_0_1_1 (h : ⟨0, 0, 1, 1⟩ ∈ G) : HasD (Hilbert.Geach α G) where
-  p := h2.vec[0]
+instance HasD_of_mem_0_0_1_1 (h : ⟨0, 0, 1, 1⟩ ∈ G) : HasD (Hilbert.Geach G) where
+  p := 0
   mem_D := by
-    unfold Hilbert.Geach;
-    simp;
+    simp [Hilbert.Geach];
     use ⟨0, 0, 1, 1⟩;
     simpa;
 
-instance HasFour_of_mem_0_2_1_0 (h : ⟨0, 2, 1, 0⟩ ∈ G) : HasFour (Hilbert.Geach α G) where
-  p := h2.vec[0]
+instance HasFour_of_mem_0_2_1_0 (h : ⟨0, 2, 1, 0⟩ ∈ G) : HasFour (Hilbert.Geach G) where
+  p := 0
   mem_Four := by
-    unfold Hilbert.Geach;
-    simp;
+    simp [Hilbert.Geach];
     use ⟨0, 2, 1, 0⟩;
     simpa;
 
-instance HasFive_of_mem_1_1_0_1 (h : ⟨1, 1, 0, 1⟩ ∈ G) : HasFive (Hilbert.Geach α G) where
-  p := h2.vec[0]
+instance HasFive_of_mem_1_1_0_1 (h : ⟨1, 1, 0, 1⟩ ∈ G) : HasFive (Hilbert.Geach G) where
+  p := 0
   mem_Five := by
-    unfold Hilbert.Geach;
-    simp;
+    simp [Hilbert.Geach];
     use ⟨1, 1, 0, 1⟩;
+    simpa;
+
+instance HasDot2_of_mem_1_1_1_1 (h : ⟨1, 1, 1, 1⟩ ∈ G) : HasDot2 (Hilbert.Geach G) where
+  p := 0
+  mem_Dot2 := by
+    simp [Hilbert.Geach];
+    use ⟨1, 1, 1, 1⟩;
+    simpa;
+
+instance HasTc_of_mem_0_1_0_0 (h : ⟨0, 1, 0, 0⟩ ∈ G) : HasTc (Hilbert.Geach G) where
+  p := 0
+  mem_Tc := by
+    simp [Hilbert.Geach];
+    use ⟨0, 1, 0, 0⟩;
     simpa;
 
 end Hilbert
