Foundation/Modal/Kripke2/Definability.lean
@@ -1,0 +1,23 @@
+import Foundation.Modal.Kripke2.Basic
+
+namespace LO.Modal
+
+namespace Kripke
+
+variable {C : Kripke.FrameClass}
+
+def FrameClass.definedBy (C : Kripke.FrameClass) (Γ : Set (Formula ℕ)) := ∀ F, F ∈ C ↔ (∀ φ ∈ Γ, F ⊧ φ)
+
+def FrameClass.definedByFormula (C : Kripke.FrameClass) (φ : Formula ℕ) := C.definedBy {φ}
+
+
+-- lemma subst_instances (definedBy : C.definedBy Γ) (h : φ ∈ Γ) : ∀ s, F ⊧ φ  := by sorry;
+
+
+def FiniteFrameClass.definedBy (C : Kripke.FiniteFrameClass) (Γ : Set (Formula ℕ)) := ∀ F, F ∈ C ↔ F.toFrame ⊧* Γ
+
+def FiniteFrameClass.definedByFormula (C : Kripke.FiniteFrameClass) (φ : Formula ℕ) := C.definedBy {φ}
+
+end Kripke
+
+end LO.Modal
