Foundation/Modal/Kripke2/Soundness.lean
@@ -1,0 +1,49 @@
+import Foundation.Modal.Hilbert2.Basic
+import Foundation.Modal.Kripke2.Definability
+
+namespace LO.Modal
+
+namespace Hilbert.Kripke
+
+variable {C : Kripke.FrameClass}
+variable {H : Hilbert ℕ} {Γ : Set (Formula ℕ)} {φ : Formula ℕ}
+
+open Formula
+open Formula.Kripke
+
+lemma soundness_of_defined_by_AxiomInstances (definedBy : C.definedBy H.axiomInstances)
+  : H ⊢! φ → C ⊧ φ := by
+  intro hφ F hF;
+  replace hφ := deductive₂_of_deductive hφ;
+  induction hφ using Deduction₂.inducition! with
+  | hMaxm h =>
+    obtain ⟨ψ, h, ⟨s, rfl⟩⟩ := h;
+    apply definedBy F |>.mp hF (ψ⟦s⟧);
+    use ψ;
+    constructor;
+    . assumption;
+    . use s;
+  | hMdp ihpq ihp => exact ValidOnFrame.mdp ihpq ihp;
+  | hNec ih => exact ValidOnFrame.nec ih;
+  | hImply₁ => exact ValidOnFrame.imply₁;
+  | hImply₂ => exact ValidOnFrame.imply₂;
+  | hElimContra => exact ValidOnFrame.elimContra;
+
+lemma defined_by_AxiomInstances_of_defined_by_Axioms (definedBy : C.definedBy H.axioms)
+  : C.definedBy H.axiomInstances := by
+  intro F;
+  constructor;
+  . rintro hC φ ⟨ψ, hs, ⟨s, rfl⟩⟩;
+    exact Kripke.ValidOnFrame.subst $ definedBy F |>.mp hC ψ hs;
+  . intro h;
+    apply definedBy F |>.mpr;
+    intro φ hφ;
+    apply h;
+    use φ;
+    constructor;
+    . assumption;
+    . use id;
+
+end Hilbert.Kripke
+
+end LO.Modal
